FStar.ListProperties verifies with --universes

src/smtencoding/encode.fs
@@ -1298,7 +1298,10 @@ and encode_sigelt' (env:env_t) (se:sigelt) : (decls_t * env_t) =
                               let binders, body, _, _ = destruct_bound_function flid t_norm e in
                               let vars, guards, env', binder_decls, _ = encode_binders None binders env in
                               let app = match vars with [] -> Term.mkFreeV(f, Term_sort) | _ -> Term.mkApp(f, List.map mkFreeV vars) in
-                              let body, decls2 = encode_term body env' in
+                              let app, (body, decls2) =
+                                 if quals |> List.contains Logic
+                                 then mk_Valid app, encode_formula body env'
+                                 else app, encode_term body env' in
                               let eqn = Term.Assume(mkForall([[app]], vars, mkImp(mk_and_l guards, mkEq(app, body))), 
                                             Some (Util.format1 "Equation for %s" flid.str)) in
                               decls@binder_decls@decls2@[eqn], env
